TBC.

spark2Cminor.v
@@ -230,10 +230,10 @@ Function make_load (addr : Cminor.expr) (ty_res : Ctypes.type) :=
     indirection of the variable of offset Zero (i.e. the pointer to
     enclosing procedure). This is the way we access to enclosing
     procedure frame. The type of all Load is ( void * ). *)
-Function build_loads_ (m:nat) {struct m} : Cminor.expr :=
+Function build_loads_ base (m:nat) {struct m} : Cminor.expr :=
   match m with
-    | O => Econst (Oaddrstack Integers.Int.zero)
-    | S m' => let subloads := build_loads_ m' in
+    | O => base
+    | S m' => let subloads := build_loads_ base m' in
               Eload AST.Mint32 subloads
   end.
 
@@ -242,7 +242,7 @@ Function build_loads_ (m:nat) {struct m} : Cminor.expr :=
     above the current frame. This is done by following pointers from
     frames to frames. (Load^m 0)+n. *)
 Definition build_loads (m:nat) (n:Z) :=
-  let indirections := build_loads_ m in
+  let indirections := build_loads_ (Econst (Oaddrstack Integers.Int.zero)) m in
   Ebinop Oadd indirections (Econst (Ointconst (Integers.Int.repr n))).
 
 
@@ -640,7 +640,7 @@ Definition transl_stmt_aux :=
            procedure. Note also that if lvl is 0, then addr_enclosing_frame
            is void (global procedures have void chaining param). This is ensured
            by the call to the main procedure below. *)
-        let addr_enclosing_frame := build_loads_ (current_lvl - lvl) in
+        let addr_enclosing_frame := build_loads_ (Econst (Oaddrstack Integers.Int.zero)) (current_lvl - lvl) in
         (* Add it as one more argument to the procedure called. *)
         do tle' <- OK (addr_enclosing_frame :: tle) ;
         (* Call the procedure; procedure name does not change (except it is a positive) ? *)
@@ -1136,6 +1136,8 @@ Ltac rename_hyp1 h th :=
 
     | build_loads ?n ?z = _ => fresh "heq_build_loads_" n "_" z
     | build_loads _ _ = _ => fresh "heq_build_loads"
+    | build_loads_ ?n ?z = _ => fresh "heq_build_loads_" n "_" z
+    | build_loads_ _ _ = _ => fresh "heq_build_loads"
     | make_load _ _ = Error _ => fresh "heq_make_load_RE"
     | make_load _ _ = _ => fresh "heq_make_load"
     | reduce_type _ _ _ = Error _ => fresh "heq_reduce_type_RE"
